theories/autosubst/AST.v
@@ -8,7 +8,7 @@ Module Core.
 Inductive term : Type :=
   | var : nat -> term
   | Sort : mode -> level -> term
-  | Pi : mode -> term -> term -> term
+  | Pi : mode -> mode -> term -> term -> term
   | lam : term -> term -> term
   | app : term -> term -> term
   | Erased : term -> term
@@ -28,13 +28,16 @@ exact (eq_trans (eq_trans eq_refl (ap (fun x => Sort x s1) H0))
          (ap (fun x => Sort t0 x) H1)).
 Qed.
 
-Lemma congr_Pi {s0 : mode} {s1 : term} {s2 : term} {t0 : mode} {t1 : term}
-  {t2 : term} (H0 : s0 = t0) (H1 : s1 = t1) (H2 : s2 = t2) :
-  Pi s0 s1 s2 = Pi t0 t1 t2.
+Lemma congr_Pi {s0 : mode} {s1 : mode} {s2 : term} {s3 : term} {t0 : mode}
+  {t1 : mode} {t2 : term} {t3 : term} (H0 : s0 = t0) (H1 : s1 = t1)
+  (H2 : s2 = t2) (H3 : s3 = t3) : Pi s0 s1 s2 s3 = Pi t0 t1 t2 t3.
 Proof.
 exact (eq_trans
-         (eq_trans (eq_trans eq_refl (ap (fun x => Pi x s1 s2) H0))
-            (ap (fun x => Pi t0 x s2) H1)) (ap (fun x => Pi t0 t1 x) H2)).
+         (eq_trans
+            (eq_trans (eq_trans eq_refl (ap (fun x => Pi x s1 s2 s3) H0))
+               (ap (fun x => Pi t0 x s2 s3) H1))
+            (ap (fun x => Pi t0 t1 x s3) H2))
+         (ap (fun x => Pi t0 t1 t2 x) H3)).
 Qed.
 
 Lemma congr_lam {s0 : term} {s1 : term} {t0 : term} {t1 : term}
@@ -130,8 +133,8 @@ Fixpoint ren_term (xi_term : nat -> nat) (s : term) {struct s} : term :=
   match s with
   | var s0 => var (xi_term s0)
   | Sort s0 s1 => Sort s0 s1
-  | Pi s0 s1 s2 =>
-      Pi s0 (ren_term xi_term s1) (ren_term (upRen_term_term xi_term) s2)
+  | Pi s0 s1 s2 s3 =>
+      Pi s0 s1 (ren_term xi_term s2) (ren_term (upRen_term_term xi_term) s3)
   | lam s0 s1 =>
       lam (ren_term xi_term s0) (ren_term (upRen_term_term xi_term) s1)
   | app s0 s1 => app (ren_term xi_term s0) (ren_term xi_term s1)
@@ -157,14 +160,14 @@ Proof.
 exact (scons (var var_zero) (funcomp (ren_term shift) sigma)).
 Defined.
 
-Fixpoint subst_term (sigma_term : nat -> term) (s : term) {struct s} :
+Fixpoint subst_term (sigma_term : nat -> term) (s : term) {struct s} : 
 term :=
   match s with
   | var s0 => sigma_term s0
   | Sort s0 s1 => Sort s0 s1
-  | Pi s0 s1 s2 =>
-      Pi s0 (subst_term sigma_term s1)
-        (subst_term (up_term_term sigma_term) s2)
+  | Pi s0 s1 s2 s3 =>
+      Pi s0 s1 (subst_term sigma_term s2)
+        (subst_term (up_term_term sigma_term) s3)
   | lam s0 s1 =>
       lam (subst_term sigma_term s0)
         (subst_term (up_term_term sigma_term) s1)
@@ -205,9 +208,9 @@ subst_term sigma_term s = s :=
   match s with
   | var s0 => Eq_term s0
   | Sort s0 s1 => congr_Sort (eq_refl s0) (eq_refl s1)
-  | Pi s0 s1 s2 =>
-      congr_Pi (eq_refl s0) (idSubst_term sigma_term Eq_term s1)
-        (idSubst_term (up_term_term sigma_term) (upId_term_term _ Eq_term) s2)
+  | Pi s0 s1 s2 s3 =>
+      congr_Pi (eq_refl s0) (eq_refl s1) (idSubst_term sigma_term Eq_term s2)
+        (idSubst_term (up_term_term sigma_term) (upId_term_term _ Eq_term) s3)
   | lam s0 s1 =>
       congr_lam (idSubst_term sigma_term Eq_term s0)
         (idSubst_term (up_term_term sigma_term) (upId_term_term _ Eq_term) s1)
@@ -256,10 +259,11 @@ ren_term xi_term s = ren_term zeta_term s :=
   match s with
   | var s0 => ap (var) (Eq_term s0)
   | Sort s0 s1 => congr_Sort (eq_refl s0) (eq_refl s1)
-  | Pi s0 s1 s2 =>
-      congr_Pi (eq_refl s0) (extRen_term xi_term zeta_term Eq_term s1)
+  | Pi s0 s1 s2 s3 =>
+      congr_Pi (eq_refl s0) (eq_refl s1)
+        (extRen_term xi_term zeta_term Eq_term s2)
         (extRen_term (upRen_term_term xi_term) (upRen_term_term zeta_term)
-           (upExtRen_term_term _ _ Eq_term) s2)
+           (upExtRen_term_term _ _ Eq_term) s3)
   | lam s0 s1 =>
       congr_lam (extRen_term xi_term zeta_term Eq_term s0)
         (extRen_term (upRen_term_term xi_term) (upRen_term_term zeta_term)
@@ -310,10 +314,11 @@ subst_term sigma_term s = subst_term tau_term s :=
   match s with
   | var s0 => Eq_term s0
   | Sort s0 s1 => congr_Sort (eq_refl s0) (eq_refl s1)
-  | Pi s0 s1 s2 =>
-      congr_Pi (eq_refl s0) (ext_term sigma_term tau_term Eq_term s1)
+  | Pi s0 s1 s2 s3 =>
+      congr_Pi (eq_refl s0) (eq_refl s1)
+        (ext_term sigma_term tau_term Eq_term s2)
         (ext_term (up_term_term sigma_term) (up_term_term tau_term)
-           (upExt_term_term _ _ Eq_term) s2)
+           (upExt_term_term _ _ Eq_term) s3)
   | lam s0 s1 =>
       congr_lam (ext_term sigma_term tau_term Eq_term s0)
         (ext_term (up_term_term sigma_term) (up_term_term tau_term)
@@ -363,12 +368,12 @@ Fixpoint compRenRen_term (xi_term : nat -> nat) (zeta_term : nat -> nat)
   match s with
   | var s0 => ap (var) (Eq_term s0)
   | Sort s0 s1 => congr_Sort (eq_refl s0) (eq_refl s1)
-  | Pi s0 s1 s2 =>
-      congr_Pi (eq_refl s0)
-        (compRenRen_term xi_term zeta_term rho_term Eq_term s1)
+  | Pi s0 s1 s2 s3 =>
+      congr_Pi (eq_refl s0) (eq_refl s1)
+        (compRenRen_term xi_term zeta_term rho_term Eq_term s2)
         (compRenRen_term (upRen_term_term xi_term)
            (upRen_term_term zeta_term) (upRen_term_term rho_term)
-           (up_ren_ren _ _ _ Eq_term) s2)
+           (up_ren_ren _ _ _ Eq_term) s3)
   | lam s0 s1 =>
       congr_lam (compRenRen_term xi_term zeta_term rho_term Eq_term s0)
         (compRenRen_term (upRen_term_term xi_term)
@@ -426,12 +431,12 @@ subst_term tau_term (ren_term xi_term s) = subst_term theta_term s :=
   match s with
   | var s0 => Eq_term s0
   | Sort s0 s1 => congr_Sort (eq_refl s0) (eq_refl s1)
-  | Pi s0 s1 s2 =>
-      congr_Pi (eq_refl s0)
-        (compRenSubst_term xi_term tau_term theta_term Eq_term s1)
+  | Pi s0 s1 s2 s3 =>
+      congr_Pi (eq_refl s0) (eq_refl s1)
+        (compRenSubst_term xi_term tau_term theta_term Eq_term s2)
         (compRenSubst_term (upRen_term_term xi_term) (up_term_term tau_term)
            (up_term_term theta_term) (up_ren_subst_term_term _ _ _ Eq_term)
-           s2)
+           s3)
   | lam s0 s1 =>
       congr_lam (compRenSubst_term xi_term tau_term theta_term Eq_term s0)
         (compRenSubst_term (upRen_term_term xi_term) (up_term_term tau_term)
@@ -500,12 +505,12 @@ ren_term zeta_term (subst_term sigma_term s) = subst_term theta_term s :=
   match s with
   | var s0 => Eq_term s0
   | Sort s0 s1 => congr_Sort (eq_refl s0) (eq_refl s1)
-  | Pi s0 s1 s2 =>
-      congr_Pi (eq_refl s0)
-        (compSubstRen_term sigma_term zeta_term theta_term Eq_term s1)
+  | Pi s0 s1 s2 s3 =>
+      congr_Pi (eq_refl s0) (eq_refl s1)
+        (compSubstRen_term sigma_term zeta_term theta_term Eq_term s2)
         (compSubstRen_term (up_term_term sigma_term)
            (upRen_term_term zeta_term) (up_term_term theta_term)
-           (up_subst_ren_term_term _ _ _ Eq_term) s2)
+           (up_subst_ren_term_term _ _ _ Eq_term) s3)
   | lam s0 s1 =>
       congr_lam
         (compSubstRen_term sigma_term zeta_term theta_term Eq_term s0)
@@ -584,12 +589,12 @@ subst_term tau_term (subst_term sigma_term s) = subst_term theta_term s :=
   match s with
   | var s0 => Eq_term s0
   | Sort s0 s1 => congr_Sort (eq_refl s0) (eq_refl s1)
-  | Pi s0 s1 s2 =>
-      congr_Pi (eq_refl s0)
-        (compSubstSubst_term sigma_term tau_term theta_term Eq_term s1)
+  | Pi s0 s1 s2 s3 =>
+      congr_Pi (eq_refl s0) (eq_refl s1)
+        (compSubstSubst_term sigma_term tau_term theta_term Eq_term s2)
         (compSubstSubst_term (up_term_term sigma_term)
            (up_term_term tau_term) (up_term_term theta_term)
-           (up_subst_subst_term_term _ _ _ Eq_term) s2)
+           (up_subst_subst_term_term _ _ _ Eq_term) s3)
   | lam s0 s1 =>
       congr_lam
         (compSubstSubst_term sigma_term tau_term theta_term Eq_term s0)
@@ -720,10 +725,11 @@ Fixpoint rinst_inst_term (xi_term : nat -> nat) (sigma_term : nat -> term)
   match s with
   | var s0 => Eq_term s0
   | Sort s0 s1 => congr_Sort (eq_refl s0) (eq_refl s1)
-  | Pi s0 s1 s2 =>
-      congr_Pi (eq_refl s0) (rinst_inst_term xi_term sigma_term Eq_term s1)
+  | Pi s0 s1 s2 s3 =>
+      congr_Pi (eq_refl s0) (eq_refl s1)
+        (rinst_inst_term xi_term sigma_term Eq_term s2)
         (rinst_inst_term (upRen_term_term xi_term) (up_term_term sigma_term)
-           (rinstInst_up_term_term _ _ Eq_term) s2)
+           (rinstInst_up_term_term _ _ Eq_term) s3)
   | lam s0 s1 =>
       congr_lam (rinst_inst_term xi_term sigma_term Eq_term s0)
         (rinst_inst_term (upRen_term_term xi_term) (up_term_term sigma_term)
@@ -898,7 +904,7 @@ Tactic Notation "auto_unfold" "in" "*" := repeat
                                            unfold VarInstance_term, Var, ids,
                                             Ren_term, Ren1, ren1,
                                             Up_term_term, Up_term, up_term,
-                                            Subst_term, Subst1, subst1
+                                            Subst_term, Subst1, subst1 
                                             in *.
 
 Ltac asimpl' := repeat (first
@@ -955,10 +961,11 @@ Fixpoint allfv_term (p_term : nat -> Prop) (s : term) {struct s} : Prop :=
   match s with
   | var s0 => p_term s0
   | Sort s0 s1 => and True (and True True)
-  | Pi s0 s1 s2 =>
+  | Pi s0 s1 s2 s3 =>
       and True
-        (and (allfv_term p_term s1)
-           (and (allfv_term (upAllfv_term_term p_term) s2) True))
+        (and True
+           (and (allfv_term p_term s2)
+              (and (allfv_term (upAllfv_term_term p_term) s3) True)))
   | lam s0 s1 =>
       and (allfv_term p_term s0)
         (and (allfv_term (upAllfv_term_term p_term) s1) True)
@@ -997,12 +1004,13 @@ Fixpoint allfvTriv_term (p_term : nat -> Prop) (H_term : forall x, p_term x)
   match s with
   | var s0 => H_term s0
   | Sort s0 s1 => conj I (conj I I)
-  | Pi s0 s1 s2 =>
+  | Pi s0 s1 s2 s3 =>
       conj I
-        (conj (allfvTriv_term p_term H_term s1)
-           (conj
-              (allfvTriv_term (upAllfv_term_term p_term)
-                 (upAllfvTriv_term_term H_term) s2) I))
+        (conj I
+           (conj (allfvTriv_term p_term H_term s2)
+              (conj
+                 (allfvTriv_term (upAllfv_term_term p_term)
+                    (upAllfvTriv_term_term H_term) s3) I)))
   | lam s0 s1 =>
       conj (allfvTriv_term p_term H_term s0)
         (conj
@@ -1054,19 +1062,12 @@ allfv_term p_term s -> allfv_term q_term s :=
   match s with
   | var s0 => fun HP => H_term s0 HP
   | Sort s0 s1 => fun HP => conj I (conj I I)
-  | Pi s0 s1 s2 =>
+  | Pi s0 s1 s2 s3 =>
       fun HP =>
       conj I
-        (conj
-           (allfvImpl_term p_term q_term H_term s1
-              match HP with
-              | conj _ HP => match HP with
-                             | conj HP _ => HP
-                             end
-              end)
+        (conj I
            (conj
-              (allfvImpl_term (upAllfv_term_term p_term)
-                 (upAllfv_term_term q_term) (upAllfvImpl_term_term H_term) s2
+              (allfvImpl_term p_term q_term H_term s2
                  match HP with
                  | conj _ HP =>
                      match HP with
@@ -1074,7 +1075,23 @@ allfv_term p_term s -> allfv_term q_term s :=
                                     | conj HP _ => HP
                                     end
                      end
-                 end) I))
+                 end)
+              (conj
+                 (allfvImpl_term (upAllfv_term_term p_term)
+                    (upAllfv_term_term q_term) (upAllfvImpl_term_term H_term)
+                    s3
+                    match HP with
+                    | conj _ HP =>
+                        match HP with
+                        | conj _ HP =>
+                            match HP with
+                            | conj _ HP =>
+                                match HP with
+                                | conj HP _ => HP
+                                end
+                            end
+                        end
+                    end) I)))
   | lam s0 s1 =>
       fun HP =>
       conj
@@ -1259,28 +1276,36 @@ allfv_term (funcomp p_term xi_term) s :=
   match s with
   | var s0 => fun H => H
   | Sort s0 s1 => fun H => conj I (conj I I)
-  | Pi s0 s1 s2 =>
+  | Pi s0 s1 s2 s3 =>
       fun H =>
       conj I
-        (conj
-           (allfvRenL_term p_term xi_term s1
-              match H with
-              | conj _ H => match H with
-                            | conj H _ => H
-                            end
-              end)
+        (conj I
            (conj
-              (allfvImpl_term _ _ (upAllfvRenL_term_term p_term xi_term) s2
-                 (allfvRenL_term (upAllfv_term_term p_term)
-                    (upRen_term_term xi_term) s2
-                    match H with
-                    | conj _ H =>
-                        match H with
-                        | conj _ H => match H with
-                                      | conj H _ => H
-                                      end
-                        end
-                    end)) I))
+              (allfvRenL_term p_term xi_term s2
+                 match H with
+                 | conj _ H =>
+                     match H with
+                     | conj _ H => match H with
+                                   | conj H _ => H
+                                   end
+                     end
+                 end)
+              (conj
+                 (allfvImpl_term _ _ (upAllfvRenL_term_term p_term xi_term)
+                    s3
+                    (allfvRenL_term (upAllfv_term_term p_term)
+                       (upRen_term_term xi_term) s3
+                       match H with
+                       | conj _ H =>
+                           match H with
+                           | conj _ H =>
+                               match H with
+                               | conj _ H => match H with
+                                             | conj H _ => H
+                                             end
+                               end
+                           end
+                       end)) I)))
   | lam s0 s1 =>
       fun H =>
       conj
@@ -1457,29 +1482,36 @@ allfv_term p_term (ren_term xi_term s) :=
   match s with
   | var s0 => fun H => H
   | Sort s0 s1 => fun H => conj I (conj I I)
-  | Pi s0 s1 s2 =>
+  | Pi s0 s1 s2 s3 =>
       fun H =>
       conj I
-        (conj
-           (allfvRenR_term p_term xi_term s1
-              match H with
-              | conj _ H => match H with
-                            | conj H _ => H
-                            end
-              end)
+        (conj I
            (conj
-              (allfvRenR_term (upAllfv_term_term p_term)
-                 (upRen_term_term xi_term) s2
-                 (allfvImpl_term _ _ (upAllfvRenR_term_term p_term xi_term)
-                    s2
-                    match H with
-                    | conj _ H =>
-                        match H with
-                        | conj _ H => match H with
-                                      | conj H _ => H
-                                      end
-                        end
-                    end)) I))
+              (allfvRenR_term p_term xi_term s2
+                 match H with
+                 | conj _ H =>
+                     match H with
+                     | conj _ H => match H with
+                                   | conj H _ => H
+                                   end
+                     end
+                 end)
+              (conj
+                 (allfvRenR_term (upAllfv_term_term p_term)
+                    (upRen_term_term xi_term) s3
+                    (allfvImpl_term _ _
+                       (upAllfvRenR_term_term p_term xi_term) s3
+                       match H with
+                       | conj _ H =>
+                           match H with
+                           | conj _ H =>
+                               match H with
+                               | conj _ H => match H with
+                                             | conj H _ => H
+                                             end
+                               end
+                           end
+                       end)) I)))
   | lam s0 s1 =>
       fun H =>
       conj
